src/Formalization/Pipeline/DG_Domain_Registration.thy
@@ -16,17 +16,19 @@ text \<open>
 \<close>
 
 interpretation ivl_reg:
-  unit_dg_exec_analysis ivl_tf ivl_tf_st
+  unit_dg_exec_analysis ivl_tf ivl_tf_st ivl_enter_st
     "TD_side_warrowing_apinis_Interp.solve" "TD_side_warrowing_apinis_Interp.solve_c"
   by unfold_locales
-     (rule ivl_is_sound_transfer ivl_tf_st_commute
+     (rule ivl_is_sound_transfer ivl_tf_st_commute ivl_enter_st_commute
+           ivl_tf_st_ret_None ivl_tf_st_ret_Some
            TD_side_warrowing_apinis_Interp.part_post_solution_of_solve_c)+
 
 interpretation sign_reg:
-  unit_dg_exec_analysis sign_tf sign_tf_st
+  unit_dg_exec_analysis sign_tf sign_tf_st sign_enter_st
     "TD_side_always_join_Interp.solve" "TD_side_always_join_Interp.solve_c"
   by unfold_locales
-     (rule sign_is_sound_transfer sign_tf_st_commute
+     (rule sign_is_sound_transfer sign_tf_st_commute sign_enter_st_commute'
+           sign_tf_st_ret_none sign_tf_st_ret_some
            TD_side_always_join_Interp.part_post_solution_of_solve_c)+
 
 end
