src/Formalization/Pipeline/Run_Analysis_Sound.thy
@@ -22,7 +22,7 @@ text \<open>
   The result is \<^emph>\<open>query-parametric\<close>: the reached program point \<open>v\<close> is existential and
   matched to where the run actually is, and the D/G collecting endpoint
   \<^verbatim>\<open>dg_post_solution_collect_sound_ltr\<close> holds at every covered
-  point, so no premature specialisation to \<^const>\<open>cfg_exit\<close> is needed.
+  point, so no premature specialisation to \<open>cfg_exit\<close> is needed.
 
   \<^bold>\<open>Why the solver step stays a one-line adapter.\<close>  The step \<open>solve_c success ->
   part_post_solution\<close> lives in the vendored locale \<^locale>\<open>TD_side_upd_rule\<close> as
@@ -40,36 +40,44 @@ begin
 lemma dg_cmb_of_eq: "dg_cmb_of S = dg_cmb"
   by (rule ext)+ (simp add: dg_cmb_of_def dg_cmb_def)
 
+lemma dg_extra_of_eq: "dg_extra_of S g = dg_extra g"
+  by (rule ext)+ (simp add: dg_extra_of_def dg_extra_def dg_enter_def)
+
 lemma dg_gen_of_eq:
   "dg_gen_of S g bot0 s0d s0g = dg_gen g bot0 s0d s0g"
-  by (simp add: dg_gen_of_def dg_gen_def dg_cmb_of_eq)
+  by (simp add: dg_gen_of_def dg_gen_def dg_cmb_of_eq dg_extra_of_eq)
 
 subsection \<open>Semantic core: abstract post-solution to source bound\<close>
 
 theorem dg_run_source_sound_abs:
   fixes Pi :: proc_table and mnm :: pname and s0 t :: store
-  assumes wf: "wf_compile_input Pi ps main"
+  assumes wf: "wf_compile_input Pi ps mnm main"
     and src: "source_com main"
+    and swf: "source_wf (main, s0, [])"
     and pp: "part_post_solution (dg_gen (compile_prog Pi ps mnm main) bot0 s0d s0g) x sigma vars"
     and cover_entry: "(cfg_entry (compile_prog Pi ps mnm main), ()) \<in> vars"
     and cover_edge:
-      "\<And>u a w. (u, a, w) \<in> edges (compile_prog Pi ps mnm main) \<Longrightarrow> (w, ()) \<in> vars"
+      "\<And>u a w. (u, a, w) \<in> intra (compile_prog Pi ps mnm main) \<Longrightarrow> (w, ()) \<in> vars"
+    and cover_enter:
+      "\<And>c dst fs as p k. (c, CallEdge dst fs as, FunctionEntry p, k) \<in> calls (compile_prog Pi ps mnm main)
+         \<Longrightarrow> (FunctionEntry p, ()) \<in> vars"
     and cover_combine:
-      "\<And>cc ex w dst. (cc, ex, w, dst) \<in> combines (compile_prog Pi ps mnm main) \<Longrightarrow> (w, ()) \<in> vars"
-    and finE: "finite (edges (compile_prog Pi ps mnm main))"
-    and finC: "finite (combines (compile_prog Pi ps mnm main))"
+      "\<And>c dst fs as p k. (c, CallEdge dst fs as, FunctionEntry p, k) \<in> calls (compile_prog Pi ps mnm main)
+         \<Longrightarrow> (k, ()) \<in> vars"
+    and finI: "finite (intra (compile_prog Pi ps mnm main))"
+    and finC: "finite (calls (compile_prog Pi ps mnm main))"
     and sound0: "S0 \<subseteq> gammaDG s0d s0g"
     and s0mem: "s0 \<in> S0"
     and run: "star (pstep Pi) (main, s0, []) (residual, t, frs)"
-  shows "\<exists>v stk. concrete_program_match Pi ps main (residual, t, frs) (v, t, stk)
+  shows "\<exists>v stk. csim Pi (compile_prog Pi ps mnm main) (residual, t, frs) (v, t, stk)
                  \<and> t \<in> dg_gamma sigma v"
 proof -
-  from source_reaches_ltr_collect[OF wf src s0mem run]
-  obtain v stk where m: "concrete_program_match Pi ps main (residual, t, frs) (v, t, stk)"
+  from source_reaches_ltr_collect[OF wf src swf s0mem run]
+  obtain v stk where m: "csim Pi (compile_prog Pi ps mnm main) (residual, t, frs) (v, t, stk)"
     and coll: "t \<in> ltr_collect (compile_prog Pi ps mnm main) S0 v" by blast
   have "ltr_collect (compile_prog Pi ps mnm main) S0 v \<subseteq> dg_gamma sigma v"
     by (rule dg_post_solution_collect_sound_ltr
-          [OF pp cover_entry cover_edge cover_combine finE finC sound0])
+          [OF pp cover_entry cover_edge cover_enter cover_combine finI finC sound0])
   then show ?thesis using m coll by blast
 qed
 
@@ -93,23 +101,30 @@ theorem dg_exec_run_source_sound:
   assumes sds: "sound_dg_spec S_abs gammaDG"
     and Hstep: "\<And>a d g. map_prod fun_of_st fun_of_st (dg_spec_step S_st a d g)
                         = dg_spec_step S_abs a (fun_of_st d) (fun_of_st g)"
+    and Henter: "\<And>xs es d g. map_prod fun_of_st fun_of_st (dgs_enter S_st xs es d g)
+                        = dgs_enter S_abs xs es (fun_of_st d) (fun_of_st g)"
     and Hcomb: "\<And>dst dc de g. map_prod fun_of_st fun_of_st (dgs_combine S_st dst dc de g)
                         = dgs_combine S_abs dst (fun_of_st dc) (fun_of_st de) (fun_of_st g)"
     and pp_st: "part_post_solution
                   (dg_gen_of S_st (compile_prog Pi ps mnm main) bot0 s0d s0g) x sigma_st vars"
-    and wf: "wf_compile_input Pi ps main"
+    and wf: "wf_compile_input Pi ps mnm main"
     and src: "source_com main"
+    and swf: "source_wf (main, s0, [])"
     and cover_entry: "(cfg_entry (compile_prog Pi ps mnm main), ()) \<in> vars"
     and cover_edge:
-      "\<And>u a w. (u, a, w) \<in> edges (compile_prog Pi ps mnm main) \<Longrightarrow> (w, ()) \<in> vars"
+      "\<And>u a w. (u, a, w) \<in> intra (compile_prog Pi ps mnm main) \<Longrightarrow> (w, ()) \<in> vars"
+    and cover_enter:
+      "\<And>c dst fs as p k. (c, CallEdge dst fs as, FunctionEntry p, k) \<in> calls (compile_prog Pi ps mnm main)
+         \<Longrightarrow> (FunctionEntry p, ()) \<in> vars"
     and cover_combine:
-      "\<And>cc ex w dst. (cc, ex, w, dst) \<in> combines (compile_prog Pi ps mnm main) \<Longrightarrow> (w, ()) \<in> vars"
-    and finE: "finite (edges (compile_prog Pi ps mnm main))"
-    and finC: "finite (combines (compile_prog Pi ps mnm main))"
+      "\<And>c dst fs as p k. (c, CallEdge dst fs as, FunctionEntry p, k) \<in> calls (compile_prog Pi ps mnm main)
+         \<Longrightarrow> (k, ()) \<in> vars"
+    and finI: "finite (intra (compile_prog Pi ps mnm main))"
+    and finC: "finite (calls (compile_prog Pi ps mnm main))"
     and sound0: "S0 \<subseteq> gammaDG (fun_of_st s0d) (fun_of_st s0g)"
     and s0mem: "s0 \<in> S0"
     and run: "star (pstep Pi) (main, s0, []) (residual, t, frs)"
-  shows "\<exists>v stk. concrete_program_match Pi ps main (residual, t, frs) (v, t, stk)
+  shows "\<exists>v stk. csim Pi (compile_prog Pi ps mnm main) (residual, t, frs) (v, t, stk)
                  \<and> t \<in> sound_dg_spec.dg_gamma gammaDG (fun_of_dg_st \<circ> sigma_st) v"
 proof -
   interpret sds: sound_dg_spec S_abs gammaDG by (rule sds)
@@ -117,7 +132,7 @@ proof -
       (dg_gen_of S_abs (compile_prog Pi ps mnm main)
          (fun_of_st bot0) (fun_of_st s0d) (fun_of_st s0g))
       x (fun_of_dg_st \<circ> sigma_st) vars"
-    by (rule part_post_solution_dg_st_to_abs[OF Hstep Hcomb pp_st])
+    by (rule part_post_solution_dg_st_to_abs[OF Hstep Henter Hcomb pp_st])
   have pp_gen: "part_post_solution
       (sds.dg_gen (compile_prog Pi ps mnm main)
          (fun_of_st bot0) (fun_of_st s0d) (fun_of_st s0g))
@@ -125,7 +140,8 @@ proof -
     using pp_abs unfolding sds.dg_gen_of_eq .
   show ?thesis
     by (rule sds.dg_run_source_sound_abs
-          [OF wf src pp_gen cover_entry cover_edge cover_combine finE finC sound0 s0mem run])
+          [OF wf src swf pp_gen cover_entry cover_edge cover_enter cover_combine
+          finI finC sound0 s0mem run])
 qed
 
 section \<open>Domain-registration layer (A2)\<close>
@@ -142,13 +158,22 @@ text \<open>
 \<close>
 
 lemma unit_dg_Hstep:
-  assumes "\<And>a s. fun_of_st (tf_st a s) = apply_tf tf a (fun_of_st s)"
-  shows "map_prod fun_of_st fun_of_st (dg_spec_step (unit_dg_spec_st tf_st) a d g)
+  assumes commute: "\<And>a s. fun_of_st (tf_st a s) = apply_tf tf a (fun_of_st s)"
+    and ret_none: "\<And>p. tf_st (EA_Ret None p) = tf_st EA_Nop"
+    and ret_some: "\<And>a p. tf_st (EA_Ret (Some a) p) = tf_st (EA_Assign ret_var a)"
+  shows "map_prod fun_of_st fun_of_st (dg_spec_step (unit_dg_spec_st tf_st enter_st) a d g)
            = dg_spec_step (unit_dg_spec tf) a (fun_of_st d) (fun_of_st g)"
-  by (simp add: dg_spec_step_unit_st dg_spec_step_unit unit_step_st_commute assms)
+  by (simp add: dg_spec_step_unit_st[OF ret_none ret_some] dg_spec_step_unit
+                unit_step_st_commute commute)
+
+lemma unit_dg_Henter:
+  assumes enter_commute: "\<And>xs es s. fun_of_st (enter_st xs es s) = tf_enter tf xs es (fun_of_st s)"
+  shows "map_prod fun_of_st fun_of_st (dgs_enter (unit_dg_spec_st tf_st enter_st) xs es d g)
+           = dgs_enter (unit_dg_spec tf) xs es (fun_of_st d) (fun_of_st g)"
+  by (simp add: unit_dg_spec_st_def unit_dg_spec_def unit_step_st_commute enter_commute)
 
 lemma unit_dg_Hcomb:
-  "map_prod fun_of_st fun_of_st (dgs_combine (unit_dg_spec_st tf_st) dst dc de g)
+  "map_prod fun_of_st fun_of_st (dgs_combine (unit_dg_spec_st tf_st enter_st) dst dc de g)
      = dgs_combine (unit_dg_spec tf) dst (fun_of_st dc) (fun_of_st de) (fun_of_st g)"
   by (simp add: unit_dg_spec_st_def unit_dg_spec_def unit_combine_step_st_commute)
 
@@ -167,6 +192,7 @@ text \<open>
 locale unit_dg_exec_analysis =
   fixes tf :: "'a::sound_domain domain_transfer"
     and tf_st :: "edge_action \<Rightarrow> 'a st \<Rightarrow> 'a st"
+    and enter_st :: "vname list \<Rightarrow> aexp list \<Rightarrow> 'a st \<Rightarrow> 'a st"
     and solve :: "(pp \<times> unit, unit, ('a st, 'a st) dg_state) eqsT
                    \<Rightarrow> pp \<times> unit
                    \<Rightarrow> (pp \<times> unit) set \<times> (pp \<times> unit + unit \<Rightarrow> ('a st, 'a st) dg_state)"
@@ -175,6 +201,9 @@ locale unit_dg_exec_analysis =
                    \<Rightarrow> ((pp \<times> unit) set \<times> (pp \<times> unit + unit \<Rightarrow> ('a st, 'a st) dg_state)) option"
   assumes tf_sound: "sound_transfer tf"
     and tf_commute: "\<And>a s. fun_of_st (tf_st a s) = apply_tf tf a (fun_of_st s)"
+    and enter_commute: "\<And>xs es s. fun_of_st (enter_st xs es s) = tf_enter tf xs es (fun_of_st s)"
+    and ret_none: "\<And>p. tf_st (EA_Ret None p) = tf_st EA_Nop"
+    and ret_some: "\<And>a p. tf_st (EA_Ret (Some a) p) = tf_st (EA_Assign ret_var a)"
     and solver_pps: "\<And>eqs x. solve_c eqs x \<noteq> None
                       \<Longrightarrow> part_post_solution eqs x (snd (solve eqs x)) (fst (solve eqs x))"
 begin
@@ -187,21 +216,26 @@ lemma sds: "sound_dg_spec (unit_dg_spec tf) gamma_unit"
 
 theorem run_source_sound:
   fixes Pi :: proc_table and ps mnm main and s0 t :: store and bot0 s0d s0g :: "'a st"
-  defines "eqs \<equiv> dg_gen_of (unit_dg_spec_st tf_st) (compile_prog Pi ps mnm main) bot0 s0d s0g"
+  defines "eqs \<equiv> dg_gen_of (unit_dg_spec_st tf_st enter_st) (compile_prog Pi ps mnm main) bot0 s0d s0g"
   assumes SOLVE: "solve_c eqs x \<noteq> None"
-    and wf: "wf_compile_input Pi ps main"
+    and wf: "wf_compile_input Pi ps mnm main"
     and src: "source_com main"
+    and swf: "source_wf (main, s0, [])"
     and cover_entry: "(cfg_entry (compile_prog Pi ps mnm main), ()) \<in> fst (solve eqs x)"
     and cover_edge:
-      "\<And>u a w. (u, a, w) \<in> edges (compile_prog Pi ps mnm main) \<Longrightarrow> (w, ()) \<in> fst (solve eqs x)"
+      "\<And>u a w. (u, a, w) \<in> intra (compile_prog Pi ps mnm main) \<Longrightarrow> (w, ()) \<in> fst (solve eqs x)"
+    and cover_enter:
+      "\<And>c dst fs as p k. (c, CallEdge dst fs as, FunctionEntry p, k) \<in> calls (compile_prog Pi ps mnm main)
+         \<Longrightarrow> (FunctionEntry p, ()) \<in> fst (solve eqs x)"
     and cover_combine:
-      "\<And>cc ex w dst. (cc, ex, w, dst) \<in> combines (compile_prog Pi ps mnm main) \<Longrightarrow> (w, ()) \<in> fst (solve eqs x)"
-    and finE: "finite (edges (compile_prog Pi ps mnm main))"
-    and finC: "finite (combines (compile_prog Pi ps mnm main))"
+      "\<And>c dst fs as p k. (c, CallEdge dst fs as, FunctionEntry p, k) \<in> calls (compile_prog Pi ps mnm main)
+         \<Longrightarrow> (k, ()) \<in> fst (solve eqs x)"
+    and finI: "finite (intra (compile_prog Pi ps mnm main))"
+    and finC: "finite (calls (compile_prog Pi ps mnm main))"
     and sound0: "S0 \<subseteq> gamma_unit (fun_of_st s0d) (fun_of_st s0g)"
     and s0mem: "s0 \<in> S0"
     and run: "star (pstep Pi) (main, s0, []) (residual, t, frs)"
-  shows "\<exists>v stk. concrete_program_match Pi ps main (residual, t, frs) (v, t, stk)
+  shows "\<exists>v stk. csim Pi (compile_prog Pi ps mnm main) (residual, t, frs) (v, t, stk)
                  \<and> t \<in> gamma (snd (solve eqs x)) v"
 proof -
   have pp_st: "part_post_solution eqs x (snd (solve eqs x)) (fst (solve eqs x))"
@@ -209,10 +243,12 @@ proof -
   show ?thesis
     unfolding gamma_def eqs_def
     by (rule dg_exec_run_source_sound
-          [OF sds unit_dg_Hstep[OF tf_commute] unit_dg_Hcomb
-              pp_st[unfolded eqs_def] wf src
+          [OF sds unit_dg_Hstep[OF tf_commute ret_none ret_some]
+              unit_dg_Henter[OF enter_commute] unit_dg_Hcomb
+              pp_st[unfolded eqs_def] wf src swf
               cover_entry[unfolded eqs_def] cover_edge[unfolded eqs_def]
-              cover_combine[unfolded eqs_def] finE finC sound0 s0mem run])
+              cover_enter[unfolded eqs_def] cover_combine[unfolded eqs_def]
+              finI finC sound0 s0mem run])
 qed
 
 end
